meta-theory/pure_beta_equivScript.sml
@@ -1,0 +1,1617 @@
+(*
+  Theorem beta_equivalence:
+    App (Lam x body) arg ≅ CA_subst x arg body
+
+  where CA_subst is the capture-avoiding substitution of the free variables "x"
+  in the expression "body" with the expression "arg"
+
+  the main theorem above state's that two beta-equivalent expressions
+  belong to the same equivalence class under the eval function.
+*)
+open HolKernel Parse boolLib bossLib term_tactic;
+open fixedPointTheory arithmeticTheory listTheory stringTheory alistTheory
+     optionTheory pairTheory ltreeTheory llistTheory bagTheory
+     BasicProvers pred_setTheory relationTheory rich_listTheory finite_mapTheory
+     dep_rewrite;
+open pure_expTheory pure_valueTheory pure_evalTheory pure_eval_lemmasTheory
+     pure_exp_lemmasTheory pure_limitTheory pure_miscTheory
+     pure_exp_relTheory pure_alpha_equivTheory pure_congruenceTheory;
+
+
+val _ = new_theory "pure_beta_equiv";
+
+
+Definition fresh_var_def:
+  fresh_var v xs = if ¬MEM v xs
+                   then v
+                   else fresh_var (v ++ "'") xs
+Termination
+  WF_REL_TAC ‘measure (λ(v,xs). (LENGTH (FLAT xs) + 1) - LENGTH v)’ \\ rw[]
+  \\ Induct_on ‘xs’ \\ fs[] \\ rpt strip_tac \\ fs[]
+End
+
+Theorem fresh_var_correctness:
+  ∀v l. ¬ MEM (fresh_var v l) l
+Proof
+  recInduct fresh_var_ind \\ rw []
+  \\ once_rewrite_tac [fresh_var_def]
+  \\ IF_CASES_TAC \\ fs[]
+QED
+
+Definition fresh_var_list_def:
+  fresh_var_list []      to_avoid = [] ∧
+  fresh_var_list (x::xs) to_avoid = let fresh = fresh_var x to_avoid;
+                                    in ((x,fresh)::fresh_var_list xs (fresh::to_avoid))
+End
+
+Theorem MAP_FST_fresh_var_list:
+  ∀ v avoid. MAP FST (fresh_var_list v avoid) = v
+Proof
+  Induct \\ fs[fresh_var_list_def,MAP]
+QED
+
+Theorem fresh_var_list_correctness:
+  ∀v l. DISJOINT (set (MAP SND (fresh_var_list v l))) (set l)
+Proof
+  Induct \\ fs[fresh_var_list_def]
+  \\ rw[] \\ fs[fresh_var_correctness]
+  \\ pop_assum (qspec_then ‘(fresh_var h l::l)’ assume_tac)
+  \\ fs[EXTENSION,DISJOINT_DEF]
+  \\ metis_tac[]
+QED
+
+Theorem fresh_var_list_distinctness:
+  ∀vars avoids. ALL_DISTINCT (MAP SND (fresh_var_list vars avoids))
+Proof
+  Induct \\ fs[fresh_var_list_def]
+  \\ rw[] \\ fs[]
+  \\ CCONTR_TAC \\ fs[]
+  \\ qspecl_then [‘vars’,‘(fresh_var h avoids::avoids)’]
+                 assume_tac fresh_var_list_correctness
+  \\ CCONTR_TAC
+  \\ fs[]
+QED
+
+Theorem perm_exp_size_lemma:
+ ∀ e. list_size char_size s = list_size char_size s'
+      ⇒ exp_size (perm_exp s s' e) = exp_size e
+Proof
+  GEN_TAC
+  \\ completeInduct_on ‘exp_size e’
+  \\ fs[PULL_FORALL]
+  \\ rw[]
+  \\ Cases_on ‘e’
+  THEN1(
+   fs[perm_exp_def, perm1_def]
+   \\ fs[exp_size_def]
+   \\ IF_CASES_TAC \\ fs[]
+   \\ IF_CASES_TAC \\ fs[]
+  )
+  THEN1(
+   fs[perm_exp_def, perm1_def]
+   \\ fs[exp_size_def]
+   \\ Induct_on ‘l’ \\ fs[]
+   \\ rw[] \\ fs[exp_size_def]
+  )
+  THEN1(
+   fs[perm_exp_def, perm1_def]
+   \\ fs[exp_size_def]
+  )
+  THEN1(
+   fs[perm_exp_def, perm1_def]
+   \\ fs[exp_size_def]
+   \\ IF_CASES_TAC \\ fs[]
+   \\ IF_CASES_TAC \\ fs[]
+  )
+  THEN1(
+   fs[perm_exp_def,exp_size_def]
+   \\ Induct_on ‘l’ \\ fs[]
+   \\ strip_tac
+   \\ fs[exp_size_def]
+   \\ rw[] \\ fs[exp_size_def]
+   \\ Cases_on ‘h’ \\ fs[] \\ fs[exp_size_def] \\ rw[]
+   \\ fs[perm_exp_def,exp_size_def,perm1_def]
+   \\ IF_CASES_TAC \\ fs[perm_exp_def,exp_size_def]
+   \\ IF_CASES_TAC \\ fs[perm_exp_def,exp_size_def]
+  )
+QED
+
+Definition exp_size'_def:
+  exp_size' (Var        a) = 1                                   ∧
+  exp_size' (Prim   a0 a1) = 1 + (op_size a0 + exp3_size' a1)    ∧
+  exp_size' (App    a0 a1) = 1 + (exp_size' a0 + exp_size' a1)   ∧
+  exp_size' (Lam    a0 a1) = 1 + (1 + exp_size' a1)              ∧
+  exp_size' (Letrec a0 a1) = 1 + (exp1_size' a0 + exp_size' a1)  ∧
+  exp1_size' [] = 0                                              ∧
+  exp1_size' (a0::a1) = 1 + (exp2_size' a0 + exp1_size' a1)      ∧
+  exp2_size' (a0, a1) = 1 + (1 + exp_size' a1)                   ∧
+  exp3_size' [] = 0                                              ∧
+  exp3_size' (a0::a1) = 1 + (exp_size' a0 + exp3_size' a1)
+End
+
+Theorem exp_size'_lemma:
+  ∀ r. MEM (q,r) l' ⇒ exp_size' r < exp1_size' l'
+Proof
+  Induct_on ‘l'’ \\ fs[] \\ Cases \\ rw[] \\ fs[exp_size'_def]
+  \\ res_tac \\ fs[]
+QED
+
+Theorem perm_exp_size'_mono:
+  ∀ s s' e. exp_size' (perm_exp s s' e) = exp_size' e
+Proof
+  rw[]
+  \\ completeInduct_on ‘exp_size' e’
+  \\ rw[]
+  \\ fs[PULL_FORALL]
+  \\ Cases_on ‘e’
+  \\ fs[exp_size'_def,perm_exp_def,perm1_def]
+  THEN1 (
+    Induct_on ‘l’ \\ fs[]
+    \\ fs[exp_size'_def,perm_exp_def,perm1_def]
+  )
+  THEN1 (
+    Induct_on ‘l’ \\ fs[]
+    \\ Cases
+    \\ fs[exp_size'_def,perm_exp_def,perm1_def]
+  )
+QED
+
+
+(**************** perm_exp lemmas ******************)
+
+Triviality perm1_MAP_set:
+ ∀ l.  set l DELETE x DELETE y ⊆ set (MAP (perm1 x y) l)
+Proof
+  Induct \\ fs[]
+  \\ strip_tac \\ rw[perm1_def]
+  \\ fs [EXTENSION,SUBSET_DEF] \\ metis_tac []
+QED
+
+Triviality subset_union_weakening_gen1:
+ A ⊆ x INSERT y INSERT B ⇒ A ⊆ x INSERT y INSERT (B ∪ C)
+Proof
+  fs [EXTENSION,SUBSET_DEF] \\ metis_tac []
+QED
+
+Triviality subset_union_weakening_gen2:
+ A ⊆ x INSERT y INSERT C ⇒ A ⊆ x INSERT y INSERT (B ∪ C)
+Proof
+  fs [EXTENSION,SUBSET_DEF] \\ metis_tac []
+QED
+
+Triviality Letrec_SUBSET_INSERT_DIFF_DISTRIBUTIVITY:
+  A ⊆ y INSERT x INSERT B ∪ D
+  ∧ E DELETE x DELETE y ⊆ C
+  ⇒
+  A DIFF C ⊆ y INSERT x INSERT ((B ∪ D) DIFF E)
+Proof
+  fs [EXTENSION,SUBSET_DEF] \\ metis_tac []
+QED
+
+Triviality subset_union_weakening:
+  A ⊆ B ⇒ (A ⊆ (B ∪ C))
+Proof
+  fs [EXTENSION,SUBSET_DEF] \\ metis_tac []
+QED
+
+Triviality DIFF_UNION_DISTRIBUTIVITY:
+  (A ∪ B) DIFF C = (A DIFF C) ∪ (B DIFF C)
+Proof
+  fs [EXTENSION,SUBSET_DEF] \\ metis_tac []
+QED
+
+Triviality  perm1_MAP_set2:
+ ∀ l. set (MAP (perm1 x y) l) DELETE x DELETE y ⊆ set l
+Proof
+  Induct \\ fs[]
+  \\ strip_tac \\ rw[perm1_def]
+  \\ fs [EXTENSION,SUBSET_DEF] \\ metis_tac []
+QED
+
+Theorem freevars_perm_exp_subset:
+  ∀ e. freevars (perm_exp x y e) ⊆ y INSERT x INSERT freevars e
+Proof
+  ho_match_mp_tac freevars_ind \\ rw[]
+  THEN1 (fs[perm_exp_def,perm1_def] \\ rw[])
+  THEN1 (
+    fs[perm_exp_def,perm1_def]
+    \\fs[MAP_MAP_o,combinTheory.o_DEF,LIST_TO_SET_FLAT]
+    \\ Induct_on ‘es’ \\ fs[]
+    \\ strip_tac \\ strip_tac
+    \\ fs[GSYM INSERT_UNION_EQ]
+    \\ rw[]
+    THEN1 (
+      irule subset_union_weakening \\ fs[]
+    )
+    \\ simp[INSERT_UNION_EQ]
+    \\ match_mp_tac (GEN_ALL subset_union_weakening_gen2) \\ fs[]
+  )
+  THEN1(
+    fs[perm_exp_def,perm1_def]
+    \\ conj_tac
+    \\ fs[EXTENSION,SUBSET_DEF] \\ metis_tac[]
+  )
+  THEN1(
+    fs[perm_exp_def,perm1_def,freevars_def]
+    \\ fs[] \\ rw[]
+    \\ fs [EXTENSION,SUBSET_DEF,MEM_FILTER] \\ TRY( metis_tac [])
+  )
+  THEN1(
+    fs[perm_exp_def]
+    \\ fs[FILTER_FLAT,FILTER_APPEND_DISTRIB,MAP_MAP_o,combinTheory.o_DEF]
+    \\ ‘(λx'. FST ((λ(x',z). (perm1 x y x',perm_exp x y z)) x')) =(perm1 x y) ∘ FST’ by (
+       fs[FUN_EQ_THM]
+       \\ Cases \\ fs[]
+    )
+    \\ fs[] \\ pop_assum kall_tac
+    \\ conj_tac
+    THEN1 (
+      fs[GSYM list_to_set_diff]
+      \\ match_mp_tac Letrec_SUBSET_INSERT_DIFF_DISTRIBUTIVITY \\ fs[]
+      \\ conj_tac
+      THEN1 ( match_mp_tac subset_union_weakening_gen1 \\ fs[])
+      \\ fs[GSYM MAP_MAP_o]
+      \\ fs[perm1_MAP_set]
+    )
+    \\ ‘(λx'. FILTER (λn. ¬MEM n (MAP (perm1 x y ∘ FST) lcs))
+                       ((λ(fn,e'). freevars e')
+                       ((λ(x',z). (perm1 x y x',perm_exp x y z)) x')))
+        =
+        FILTER (λn. ¬MEM n (MAP (perm1 x y ∘ FST) lcs))
+        ∘ freevars
+        ∘ (perm_exp x y)
+        ∘ SND ’ by (
+       fs[FUN_EQ_THM]
+       \\ Cases \\ rw[]
+    ) \\ fs[] \\ pop_assum kall_tac
+    \\ fs[MAP_FILTER]
+    \\ fs[GSYM MAP_MAP_o]
+    \\ fs[GSYM FILTER_FLAT]
+    \\ fs[GSYM list_to_set_diff]
+    \\ match_mp_tac Letrec_SUBSET_INSERT_DIFF_DISTRIBUTIVITY  \\ fs[]
+    \\ reverse (rw[]) THEN1 (fs[perm1_MAP_set])
+    \\ match_mp_tac subset_union_weakening_gen2 \\ fs[]
+    \\ fs[MAP_MAP_o,LIST_TO_SET_FLAT]
+    \\ fs[BIGUNION_SUBSET]
+    \\ fs[MEM_MAP]
+    \\ strip_tac \\ rw[]
+    \\ Cases_on ‘y'’ \\ fs[]
+    \\ match_mp_tac SUBSET_TRANS
+    \\ qexists_tac ‘ y INSERT x INSERT freevars r’
+    \\ conj_tac THEN1 (res_tac \\ fs[])
+    \\ fs[]
+    \\ res_tac
+    \\ ‘set (MAP (λ(fn,e). freevars e) lcs) = set (MAP set (MAP (freevars o SND) lcs))’by(
+      ntac 4 (pop_assum kall_tac)
+      \\ Induct_on ‘lcs’ \\ fs[]
+      \\ Cases \\ fs[]
+    )
+    \\ fs[] \\ pop_assum kall_tac
+    \\ fs[GSYM LIST_TO_SET_FLAT]
+    \\ fs[SUBSET_INSERT_DELETE]
+    \\ Induct_on ‘lcs’ \\ fs[MEM]
+    \\ rw[]
+    \\ res_tac \\ fs[]
+    \\ TRY (Cases_on ‘h’) \\ rw[]
+    \\ fs [EXTENSION,SUBSET_DEF] \\ metis_tac []
+  )
+QED
+
+Theorem freevars_perm_exp_subset_inv:
+  ∀e. freevars e ⊆ y INSERT x INSERT freevars (perm_exp x y e)
+Proof
+  ho_match_mp_tac freevars_ind \\ rw[]
+  THEN1 (fs[perm_exp_def,perm1_def] \\ rw[])
+  THEN1 (
+    fs[perm_exp_def,perm1_def]
+    \\fs[MAP_MAP_o,combinTheory.o_DEF,LIST_TO_SET_FLAT]
+    \\ Induct_on ‘es’ \\ fs[]
+    \\ strip_tac \\ strip_tac
+    \\ fs[GSYM INSERT_UNION_EQ]
+    \\ rw[]
+    THEN1 (
+      irule subset_union_weakening \\ fs[]
+    )
+    \\ simp[INSERT_UNION_EQ]
+    \\ fs[EXTENSION,SUBSET_DEF] \\ metis_tac[]
+  )
+  THEN1(
+    fs[perm_exp_def,perm1_def]
+    \\ fs[EXTENSION,SUBSET_DEF] \\ metis_tac[]
+  )
+  THEN1(
+    fs[perm_exp_def,perm1_def]
+    \\ fs[EXTENSION,SUBSET_DEF] \\ metis_tac[]
+  )
+  THEN1(
+    fs[perm_exp_def,perm1_def,freevars_def]
+    \\ fs[] \\ rw[]
+    \\ fs [EXTENSION,SUBSET_DEF,MEM_FILTER] \\ TRY( metis_tac [])
+  )
+  THEN1(
+    fs[perm_exp_def]
+    \\ fs[FILTER_FLAT,FILTER_APPEND_DISTRIB,MAP_MAP_o,combinTheory.o_DEF]
+    \\ ‘(λx'. FST ((λ(x',z). (perm1 x y x',perm_exp x y z)) x')) = (perm1 x y) ∘ FST’ by (
+       fs[FUN_EQ_THM]
+       \\ Cases \\ fs[]
+    )
+    \\ fs[] \\ pop_assum kall_tac
+    \\ ‘(λx'. FILTER (λn. ¬MEM n (MAP (perm1 x y ∘ FST) lcs))
+                       ((λ(fn,e'). freevars e')
+                       ((λ(x',z). (perm1 x y x',perm_exp x y z)) x')))
+        =
+        FILTER (λn. ¬MEM n (MAP (perm1 x y ∘ FST) lcs))
+        ∘ freevars
+        ∘ (perm_exp x y)
+        ∘ SND ’ by (
+       fs[FUN_EQ_THM]
+       \\ Cases \\ rw[]
+    ) \\ fs[] \\ pop_assum kall_tac
+    \\ fs[MAP_FILTER]
+    \\ fs[GSYM MAP_MAP_o]
+    \\ fs[GSYM FILTER_FLAT]
+    \\ fs[GSYM list_to_set_diff]
+    \\ fs[DIFF_UNION_DISTRIBUTIVITY]
+    \\ conj_tac
+    THEN1 (
+      fs[GSYM DIFF_UNION_DISTRIBUTIVITY]
+      \\ match_mp_tac Letrec_SUBSET_INSERT_DIFF_DISTRIBUTIVITY  \\ fs[]
+      \\ conj_tac
+      THEN1 (match_mp_tac subset_union_weakening_gen1 \\ fs[])
+      \\ fs[perm1_MAP_set2]
+    )
+    \\ fs[GSYM DIFF_UNION_DISTRIBUTIVITY]
+    \\ match_mp_tac Letrec_SUBSET_INSERT_DIFF_DISTRIBUTIVITY  \\ fs[]
+    \\ reverse (rw[]) THEN1 (fs[perm1_MAP_set2])
+    \\ match_mp_tac subset_union_weakening_gen2 \\ fs[]
+    \\ fs[MAP_MAP_o] \\ fs[GSYM LIST_TO_SET_FLAT]
+    \\ fs[BIGUNION_SUBSET]
+    \\ fs[MEM_MAP]
+    \\ fs[GSYM UNION_SUBSET]
+    \\ strip_tac \\ rw[]
+    \\ Cases_on ‘y'’ \\ fs[]
+    \\ res_tac
+    \\ match_mp_tac SUBSET_TRANS
+    \\ qexists_tac ‘ y INSERT x INSERT freevars (perm_exp x y r)’
+    \\ conj_tac THEN1 (fs [EXTENSION,SUBSET_DEF] \\ metis_tac[])
+    \\ fs[GSYM LIST_TO_SET_FLAT]
+    \\ fs[SUBSET_INSERT_DELETE]
+    \\ Induct_on ‘lcs’ \\ fs[MEM]
+    \\ rw[]
+    \\ res_tac \\ fs[]
+    \\ fs [EXTENSION,SUBSET_DEF] \\ metis_tac []
+  )
+QED
+
+Theorem freevar_perm_exp_MEM:
+ ∀ e. MEM x (freevars e) ⇒ MEM y (freevars (perm_exp x y e))
+Proof
+  ho_match_mp_tac freevars_ind
+  \\ rpt conj_tac
+  THEN1( fs[perm_exp_def,perm1_def] \\ rw[])
+  THEN1(
+     rw[] \\ fs[MEM_MAP] \\ rw[]
+     \\ res_tac
+     \\ fs[freevars_def,perm_exp_def,perm1_def]
+     \\ fs[MEM_FLAT]
+     \\ qexists_tac ‘(freevars (perm_exp x y e))’ \\ fs[]
+     \\ fs[MAP_MAP_o,combinTheory.o_DEF]
+     \\ fs[MEM_MAP]
+     \\ qexists_tac ‘e’ \\ fs[]
+  )
+  THEN1(rw[] \\ fs[perm_exp_def,perm1_def])
+  THEN1(
+    fs[perm_exp_def,perm1_def]
+    \\ rw[] \\ fs[MEM_FILTER]
+  )
+  THEN1(
+    rpt strip_tac
+    \\ fs[freevars_def,perm_exp_def,perm1_def]
+    THEN1 (
+      fs[MEM_FILTER]
+      \\ fs[MAP_MAP_o,combinTheory.o_DEF]
+      \\ CCONTR_TAC \\ fs[]
+      \\ fs[MEM_MAP]
+      \\ Cases_on ‘x'’ \\ fs[]
+      \\ Cases_on ‘q = x’ \\ fs[]
+      THEN1 (first_assum (qspec_then ‘(x,r)’ assume_tac) \\ fs[])
+      \\ Cases_on ‘q = y’ \\ fs[]
+   )
+   \\ fs[MEM_FILTER]
+   \\ fs[MAP_MAP_o,combinTheory.o_DEF]
+   \\ fs[MEM_MAP]
+   \\ CCONTR_TAC \\ fs[]
+   THEN1 (
+     Cases_on ‘x'’ \\ fs[]
+     \\ Cases_on ‘q = x’ \\ rw[] \\ fs[]
+     \\ first_assum (qspec_then ‘(q,r)’ assume_tac) \\ rw[] \\ fs[]
+     \\ Cases_on ‘q = y’ \\ fs[]
+   )
+   \\ rw[]
+   \\ fs[MEM_MAP]
+   \\ fs[MEM_FLAT]
+   \\ fs[MEM_MAP]
+   \\ Cases_on ‘y'’ \\ res_tac \\ fs[] \\ res_tac \\ fs[]
+   \\ first_x_assum (qspec_then ‘freevars (perm_exp x y r)’ assume_tac) \\ rw[] \\ fs[]
+   \\ first_x_assum (qspec_then ‘(q,r)’ assume_tac) \\ rw[] \\ fs[]
+  )
+QED
+
+Theorem freevar_perm_exp_not_MEM:
+ ∀ e. ¬MEM x (freevars e) ⇒ ¬ MEM y (freevars (perm_exp x y e))
+Proof
+  ho_match_mp_tac freevars_ind
+  \\ rpt conj_tac
+  THEN1( fs[perm_exp_def,perm1_def] \\ rw[])
+  THEN1(
+    rw[]
+    \\ fs[MEM_MAP]
+    \\ fs[freevars_def,perm_exp_def,perm1_def]
+    \\ fs[MEM_FLAT]
+    \\ fs[MAP_MAP_o,combinTheory.o_DEF]
+    \\ fs[MEM_MAP]
+    \\ CCONTR_TAC \\ fs[] \\ rw[]
+    \\ res_tac
+    \\ first_assum (qspec_then ‘set (freevars a)’ assume_tac)
+    \\ fs[] \\ fs[]
+    \\ pop_assum (qspec_then ‘a’ assume_tac) \\ fs[]
+  )
+  THEN1(rw[] \\ fs[perm_exp_def,perm1_def])
+  THEN1(
+    fs[perm_exp_def,perm1_def]
+    \\ rw[] \\ fs[MEM_FILTER]
+  )
+  THEN1(
+    fs[freevars_def,perm_exp_def,perm1_def]
+    \\ rw[]
+    THEN1 (
+      fs[MEM_FILTER,MEM_FLAT,MEM_MAP,MAP_MAP_o,combinTheory.o_DEF]
+      \\ CCONTR_TAC \\ fs[] \\ rw[] \\ fs[]
+      \\ Cases_on ‘y''’ \\ rw[] \\ fs[]
+      \\ res_tac
+      \\ Cases_on ‘MEM x (freevars r)’ \\ fs[]
+      \\ last_x_assum (qspec_then ‘freevars r’ assume_tac) \\ rw[] \\ fs[]
+      \\ pop_assum (qspec_then ‘(q,r)’ assume_tac) \\ rw[] \\ fs[]
+    )
+    \\ fs[GSYM perm1_def]
+    \\ fs[MEM_FILTER]
+    \\ fs[MAP_MAP_o,combinTheory.o_DEF] \\ rw[]
+    \\ disj1_tac
+    \\ ‘(λx'. FST ((λ(x',z). (perm1 x y x',perm_exp x y z)) x')) = (perm1 x y) o FST’ by (
+       fs[FUN_EQ_THM]
+       \\ Cases \\ rw[]
+    )
+    \\ fs[] \\ pop_assum kall_tac
+    \\ fs[MEM_MAP]
+    \\ qexists_tac ‘y'’ \\ fs[]
+    \\ Cases_on ‘y'’ \\ fs[perm1_def]
+  )
+QED
+
+Theorem freevars_perm_exp:
+  freevars (perm_exp x y e) =
+     freevars e
+     DIFF (if x ∉ freevars e then {y} else ∅)
+     DIFF (if y ∉ freevars e then {x} else ∅)
+     ∪ (if x ∈ freevars e then {y} else ∅)
+     ∪ (if y ∈ freevars e then {x} else ∅)
+Proof
+  rw[]
+  \\ assume_tac (GEN_ALL freevars_perm_exp_subset)
+  \\ assume_tac (GEN_ALL freevars_perm_exp_subset_inv)
+  \\ assume_tac (GEN_ALL freevar_perm_exp_MEM)
+  \\ assume_tac (GEN_ALL freevar_perm_exp_not_MEM)
+  \\ TRY (fs [EXTENSION,SUBSET_DEF] \\ metis_tac [perm_exp_sym])
+QED
+
+Theorem boundvars_perm_exp_subset:
+  ∀ e.
+  boundvars (perm_exp x y e) ⊆ x INSERT y INSERT (boundvars e)
+Proof
+  recInduct boundvars_ind
+  \\ rw[]
+  THEN1 (fs[perm_exp_def])
+  THEN1 (
+    fs[perm_exp_def]
+    \\ fs[MAP_MAP_o,combinTheory.o_DEF]
+    \\ fs[LIST_TO_SET_FLAT]
+    \\ fs[MAP_MAP_o,combinTheory.o_DEF]
+    \\ fs[MEM_MAP]
+    \\ fs[BIGUNION_SUBSET]
+    \\ rw[]
+    \\ fs[MEM_MAP]
+    \\ last_assum (qspec_then ‘a’ assume_tac)
+    \\ res_tac \\ fs[]
+    \\ irule SUBSET_TRANS
+    \\ qexists_tac ‘ x INSERT y INSERT boundvars a’
+    \\ fs[]
+    \\ irule SUBSET_INSERT_RIGHT
+    \\ irule SUBSET_INSERT_RIGHT
+    \\ irule SUBSET_BIGUNION_I
+    \\ fs[MEM_MAP]
+    \\ qexists_tac ‘a’ \\ fs[]
+  )
+  THEN1 (
+    fs[perm_exp_def]
+    \\ fs[DISJOINT_SYM]
+    \\ fs[EXTENSION,SUBSET_DEF] \\ metis_tac[]
+  )
+  THEN1 (
+    fs[perm_exp_def,boundvars_def,perm1_def]
+    \\ rw[]
+    \\ fs[EXTENSION,SUBSET_DEF] \\ metis_tac[]
+  )
+  \\ fs[perm_exp_def]
+  \\ reverse conj_tac
+  THEN1 (fs[EXTENSION,SUBSET_DEF] \\ metis_tac[])
+  \\ fs[MAP_MAP_o,combinTheory.o_DEF]
+  \\ fs[LIST_TO_SET_FLAT]
+  \\ fs[MAP_MAP_o,combinTheory.o_DEF]
+  \\ fs[MEM_MAP]
+  \\ fs[BIGUNION_SUBSET]
+  \\ rw[]
+  \\ fs[MEM_MAP]
+  \\ Cases_on ‘x'’
+  \\ fs[perm1_def]
+  \\ reverse conj_tac
+  THEN1 (
+     rw[]
+     \\ res_tac
+     \\ irule SUBSET_TRANS
+     \\ qexists_tac ‘x INSERT y INSERT
+                     BIGUNION (set (MAP (λ(fn,e). fn INSERT boundvars e) lcs))’
+     \\ reverse conj_tac
+     THEN1 (fs[EXTENSION,SUBSET_DEF,UNION_DEF] \\ metis_tac[])
+     \\ fs[SUBSET_INSERT_DELETE]
+     \\ irule SUBSET_TRANS
+     \\ qexists_tac ‘q INSERT boundvars r’
+     \\ conj_tac
+     THEN1 (fs[EXTENSION,SUBSET_DEF,UNION_DEF] \\ metis_tac[])
+     \\ irule SUBSET_BIGUNION_I
+     \\ fs[MEM_MAP]
+     \\ qexists_tac ‘(q,r)’ \\ fs[]
+  )
+  \\ rw[]
+  \\ disj2_tac
+  \\ qexists_tac ‘q INSERT boundvars r’
+  \\ fs[]
+  \\ fs[MEM_MAP]
+  \\ qexists_tac ‘(q,r)’ \\ fs[]
+QED
+
+Theorem boundvars_perm_exp_subset_inv:
+  ∀e. boundvars e ⊆ x INSERT y INSERT boundvars (perm_exp x y e)
+Proof
+  recInduct boundvars_ind
+  \\ rw[]
+  THEN1 (
+    fs[perm_exp_def]
+    \\ fs[MAP_MAP_o,combinTheory.o_DEF]
+    \\ fs[LIST_TO_SET_FLAT]
+    \\ fs[MAP_MAP_o,combinTheory.o_DEF]
+    \\ fs[MEM_MAP]
+    \\ fs[BIGUNION_SUBSET]
+    \\ rw[]
+    \\ fs[MEM_MAP]
+    \\ res_tac
+    \\ irule SUBSET_TRANS
+    \\ qexists_tac ‘ x INSERT y INSERT boundvars (perm_exp x y e)’
+    \\ fs[]
+    \\ irule SUBSET_INSERT_RIGHT
+    \\ irule SUBSET_INSERT_RIGHT
+    \\ irule SUBSET_BIGUNION_I
+    \\ fs[MEM_MAP]
+    \\ qexists_tac ‘e’ \\ fs[]
+  )
+  THEN1 (
+    fs[perm_exp_def]
+    \\ fs[EXTENSION,SUBSET_DEF] \\ metis_tac[]
+  )
+  THEN1 (
+    fs[perm_exp_def]
+    \\ fs[EXTENSION,SUBSET_DEF] \\ metis_tac[]
+  )
+  THEN1 (
+    fs[perm_exp_def]
+    \\ fs[perm1_def]
+    \\ rw[]
+  )
+  THEN1 (
+    fs[perm_exp_def]
+    \\ fs[perm1_def]
+    \\ rw[]
+    \\ fs[EXTENSION,SUBSET_DEF] \\ metis_tac[]
+  )
+  THEN1 (
+    fs[perm_exp_def]
+    \\ fs[MAP_MAP_o,combinTheory.o_DEF]
+    \\ fs[LIST_TO_SET_FLAT]
+    \\ fs[MAP_MAP_o,combinTheory.o_DEF]
+    \\ fs[EXTENSION,UNION_DEF,SUBSET_DEF] \\ metis_tac[]
+  )
+  \\ fs[perm_exp_def]
+  \\ fs[MAP_MAP_o,combinTheory.o_DEF]
+  \\ fs[LIST_TO_SET_FLAT]
+  \\ fs[MAP_MAP_o,combinTheory.o_DEF]
+  \\ fs[BIGUNION_SUBSET]
+  \\ rw[]
+  \\ fs[MEM_MAP]
+  \\ Cases_on ‘y'’
+  \\ fs[perm1_def]
+  \\ rw[]
+  THEN1 (
+    CCONTR_TAC \\ fs[] \\ res_tac \\ fs[MEM_MAP]
+    \\ first_assum (qspec_then ‘q INSERT (boundvars (perm_exp x y r))’ assume_tac) \\ fs[]
+    \\ first_assum (qspec_then ‘(q,r)’ assume_tac) \\ fs[]
+    \\ pop_assum mp_tac \\ rw[]
+  )
+  \\ res_tac
+  \\ fs[SUBSET_INSERT_DELETE]
+  \\ irule SUBSET_TRANS
+  \\ qexists_tac ‘perm1 x y q INSERT boundvars (perm_exp x y r)’
+  \\ conj_tac THEN1 (fs[EXTENSION,SUBSET_DEF] \\ metis_tac[])
+  \\ irule subset_union_weakening
+  \\ irule SUBSET_BIGUNION_I
+  \\ fs[MEM_MAP]
+  \\ qexists_tac ‘(q,r)’ \\ fs[perm1_def] \\ rw[]
+QED
+
+Theorem boundvar_perm_exp_MEM:
+ ∀ e. MEM x (boundvars e) ⇒ MEM y (boundvars (perm_exp x y e))
+Proof
+  ho_match_mp_tac boundvars_ind
+  \\ rw[]
+  \\ fs[perm_exp_def]
+  \\ fs[perm1_def]
+  THEN1 (
+    fs[MAP_MAP_o,combinTheory.o_DEF]
+    \\ fs[MEM_FLAT]
+    \\ fs[MEM_MAP]
+    \\ rw[]
+    \\ res_tac
+    \\ qexists_tac ‘boundvars (perm_exp x y e)’
+    \\ rw[]
+    \\ qexists_tac ‘e’
+    \\ fs[]
+  )
+  \\ fs[GSYM perm1_def]
+  \\ fs[MAP_MAP_o,combinTheory.o_DEF]
+  \\ fs[MEM_FLAT]
+  \\ fs[MEM_MAP]
+  \\ rw[]
+  \\ Cases_on ‘y'’
+  \\ res_tac \\ fs[] \\ rw[]
+  THEN1 (
+    disj1_tac
+    \\ qexists_tac ‘y::(boundvars (perm_exp q y r))’
+    \\ fs[] \\ rw[]
+    \\ qexists_tac ‘(q,r)’
+    \\ fs[] \\ rw[]
+    \\ fs[perm1_def]
+  )
+  \\ res_tac \\ fs[] \\ rw[]
+  \\ disj1_tac
+  \\ Cases_on ‘MEM y (boundvars (perm_exp x y e))’ \\ fs[]
+  \\ qexists_tac ‘perm1 x y q::(boundvars (perm_exp x y r))’
+  \\ fs[] \\ rw[]
+  \\ qexists_tac ‘(q,r)’
+  \\ fs[] \\ rw[]
+QED
+
+Theorem boundvar_perm_exp_not_MEM:
+ ∀ e. ¬MEM x (boundvars e) ⇒ ¬ MEM y (boundvars (perm_exp x y e))
+Proof
+  ho_match_mp_tac boundvars_ind
+  \\ rw[]
+  \\ fs[perm_exp_def]
+  \\ fs[perm1_def]
+  THEN1 (
+    fs[MAP_MAP_o,combinTheory.o_DEF]
+    \\ fs[MEM_FLAT]
+    \\ fs[MEM_MAP]
+    \\ CCONTR_TAC \\ fs[]
+    \\ res_tac \\ rw[]
+    \\ Cases_on ‘MEM x (boundvars a)’ \\ fs[]
+    \\ first_assum (qspec_then ‘boundvars a’ assume_tac) \\ fs[] \\ fs[]
+    \\ metis_tac[]
+  )
+  THEN1 (
+    IF_CASES_TAC \\ fs[]
+  )
+  \\ fs[GSYM perm1_def]
+  \\ fs[MAP_MAP_o,combinTheory.o_DEF]
+  \\ fs[MEM_FLAT]
+  \\ fs[MEM_MAP]
+  \\ rw[]
+  \\ CCONTR_TAC \\ fs[]
+  \\ Cases_on ‘x'’ \\ fs[] \\ rw[]
+  \\ res_tac \\ fs[] \\ rw[]
+  THEN1 (
+    fs[perm1_def]
+    \\ pop_assum mp_tac
+    \\ pop_assum mp_tac
+    \\ IF_CASES_TAC \\ fs[]
+    \\ rw[] \\ res_tac \\ fs[]
+    \\ first_assum (qspec_then ‘q INSERT boundvars r’ assume_tac) \\ fs[]
+    \\ first_assum (qspec_then ‘(q,r)’ assume_tac) \\ fs[]
+  )
+  \\ Cases_on ‘MEM x (boundvars r)’ \\ fs[]
+  \\ first_assum (qspec_then ‘q INSERT boundvars r’ assume_tac) \\ fs[]
+  \\ fs[] \\ rw[]
+  \\ first_assum (qspec_then ‘(q,r)’ assume_tac) \\ fs[]
+QED
+
+Theorem boundvars_perm_exp:
+  boundvars (perm_exp x y e) =
+     boundvars e
+     DIFF (if x ∉ boundvars e then {y} else ∅)
+     DIFF (if y ∉ boundvars e then {x} else ∅)
+     ∪ (if x ∈ boundvars e then {y} else ∅)
+     ∪ (if y ∈ boundvars e then {x} else ∅)
+Proof
+  rw[]
+  \\ assume_tac (GEN_ALL boundvars_perm_exp_subset)
+  \\ assume_tac (GEN_ALL boundvars_perm_exp_subset_inv)
+  \\ assume_tac (GEN_ALL boundvar_perm_exp_MEM)
+  \\ assume_tac (GEN_ALL boundvar_perm_exp_not_MEM)
+  \\ fs [EXTENSION,SUBSET_DEF] \\ metis_tac [perm_exp_sym]
+QED
+
+
+(*******************)
+
+
+
+Definition perm_exp_list_def:
+  perm_exp_list [] e = e ∧
+  perm_exp_list ((old,new)::binds) e = perm_exp_list binds (perm_exp old new e)
+End
+
+Theorem perm_exp_list_size'_mono:
+  ∀ binds e. exp_size' (perm_exp_list binds e) = exp_size' e
+Proof
+  recInduct perm_exp_list_ind
+  \\ rw[] \\ fs[perm_exp_list_def,perm_exp_size'_mono]
+QED
+
+Theorem exp_alpha_perm_exp_list:
+  ∀ binds e.
+      (DISJOINT (set (MAP FST binds)) (freevars e))
+    ∧ (DISJOINT (set (MAP SND binds)) (freevars e))
+    ⇒ exp_alpha e (perm_exp_list binds e)
+Proof
+  recInduct perm_exp_list_ind
+  \\ conj_tac
+  THEN1 (
+    rw[]
+    \\ fs[perm_exp_list_def]
+    \\ fs[exp_alpha_refl]
+  )
+  \\ rw[]
+  \\ fs[perm_exp_list_def]
+  \\ irule exp_alpha_Trans
+  \\ qexists_tac  ‘(perm_exp old new e)’
+  \\ conj_tac
+  THEN1 (irule exp_alpha_perm_irrel \\ fs[])
+  \\ last_assum irule
+  \\ fs[freevars_perm_exp]
+  \\ fs[EXTENSION,DISJOINT_DEF] \\  metis_tac[]
+QED
+
+Theorem exp_alpha_perm_exp_list_trans:
+  ∀ binds e e'.
+      (DISJOINT (set (MAP FST binds)) (freevars e'))
+    ∧ (DISJOINT (set (MAP SND binds)) (freevars e'))
+    ∧ exp_alpha e e'
+    ⇒ exp_alpha e (perm_exp_list binds e')
+Proof
+  recInduct perm_exp_list_ind
+  \\ conj_tac
+  THEN1 (fs[perm_exp_list_def])
+  \\ rw[]
+  \\ fs[perm_exp_list_def]
+  \\ irule exp_alpha_Trans
+  \\ qexists_tac ‘(perm_exp old new e')’
+  \\ conj_tac
+  THEN1 (
+    irule exp_alpha_Trans
+    \\ qexists_tac ‘e'’
+    \\ fs[]
+    \\ irule exp_alpha_perm_irrel \\ fs[]
+  )
+  \\ irule exp_alpha_perm_exp_list \\ fs[]
+  \\ fs[freevars_perm_exp]
+  \\ fs[EXTENSION,DISJOINT_DEF] \\  metis_tac[]
+QED
+
+Triviality FILTER_MEM_INTERSECTION:
+  ∀ l1 l2. set (FILTER (λx. MEM x l2) l1) = set l1 ∩ set l2
+Proof
+  Induct \\ fs[]
+  \\ rw[]
+  \\ fs[EXTENSION,INTER_DEF] \\ metis_tac[]
+QED
+
+Triviality DISJOINT_UNION_DIFF:
+   DISJOINT A (B DIFF D)
+ ∧ DISJOINT A (C DIFF D) ⇒ DISJOINT A (B ∪ C DIFF D)
+Proof
+ fs[EXTENSION,DISJOINT_DEF] \\ metis_tac[]
+QED
+
+Triviality DIFF_SUBSET_UNION:
+  A DIFF B ⊆ C ⇒ A ⊆ C ∪ B
+Proof
+  fs[EXTENSION,DISJOINT_DEF,SUBSET_DEF] \\ metis_tac[]
+QED
+
+Triviality UNION_SYM:
+  ∀ A B. A ∪ B = B ∪ A
+Proof
+  fs[EXTENSION,UNION_DEF] \\ metis_tac[]
+QED
+
+Definition avoid_vars_def:
+  avoid_vars avoid (Var x) = (Var x) ∧
+  avoid_vars avoid (Prim op es) = Prim op (MAP (avoid_vars avoid) es) ∧
+  avoid_vars avoid (Lam x e) = (
+                 let fresh = fresh_var x avoid in
+                 let e'    = avoid_vars (x::fresh::avoid) e
+                 in (if MEM x avoid
+                      then Lam fresh (perm_exp x fresh e')
+                      else Lam x e'))                                ∧
+  avoid_vars avoid (App e1 e2) = App (avoid_vars avoid e1)
+                                     (avoid_vars avoid e2)           ∧
+  avoid_vars avoid (Letrec lcs e) =
+     let clashes     = nub (FILTER (λx. MEM x avoid) (MAP FST lcs))  in
+     let freshes     = fresh_var_list clashes (MAP FST lcs ++ avoid) in
+     let new_avoids  = MAP FST lcs ++ avoid ++ MAP SND freshes       in
+     let lcs_bodies' = MAP (\x. avoid_vars new_avoids (SND x)) lcs   in
+     (* let lcs_bodies' = MAP ((avoid_vars new_avoids) o SND) lcs       in *)
+     let lcs'        = ZIP (MAP FST lcs,lcs_bodies')                 in
+     let body'       = avoid_vars new_avoids e
+     in  perm_exp_list freshes (Letrec lcs' body')
+Termination
+  WF_REL_TAC ‘measure (exp_size' o SND)’ \\ fs[exp_size'_def]
+  \\ reverse (rpt conj_tac)
+  THEN1 (
+    rw[]
+    \\ Induct_on ‘es’ \\ fs[]
+    \\ rw[] \\ fs[exp_size'_def]
+  )
+  \\ rw[]
+  \\ imp_res_tac exp_size'_lemma \\ fs[]
+End
+
+Theorem exp_alpha_avoid_vars:
+  ∀ avoid e. freevars e ⊆ (set avoid) ⇒ exp_alpha e (avoid_vars avoid e)
+Proof
+  recInduct avoid_vars_ind
+  \\ rw[]
+  THEN1 (
+    fs[avoid_vars_def]
+    \\ fs[exp_alpha_refl]
+  )
+  THEN1 (
+    fs[avoid_vars_def]
+    \\ irule exp_alpha_Prim
+    \\ fs[EVERY2_EVERY]
+    \\ fs[ZIP_MAP]
+    \\ fs[EVERY_MEM]
+    \\ Cases
+    \\ fs[MAP_MAP_o,combinTheory.o_DEF]
+    \\ fs[MEM_MAP] \\ rw[]
+    \\ res_tac \\ fs[]
+    \\ pop_assum irule
+    \\ irule SUBSET_TRANS
+    \\ qexists_tac ‘BIGUNION (set (MAP (λe. freevars e) es))’
+    \\ fs[]
+    \\ fs[EXTENSION,BIGUNION,SUBSET_DEF] \\ rw[]
+    \\ qexists_tac ‘freevars q’ \\ fs[]
+    \\ fs[MEM_MAP]
+    \\ qexists_tac ‘q’ \\ fs[]
+  )
+  THEN1 (
+    fs[avoid_vars_def]
+    \\ IF_CASES_TAC
+    THEN1 (
+      ‘freevars e ⊆ set avoid’ by (fs[EXTENSION,SUBSET_DEF] \\ metis_tac[])
+      \\ res_tac \\ fs[]
+      \\ irule exp_alpha_Trans
+      \\ qexists_tac ‘Lam (fresh_var x avoid) (perm_exp x (fresh_var x avoid) e)’
+      \\ conj_tac
+      THEN1 (
+        irule exp_alpha_Alpha
+        \\ qspecl_then [‘x’,‘avoid’] assume_tac fresh_var_correctness
+        \\ fs[EXTENSION,SUBSET_DEF] \\ metis_tac[]
+      )
+      \\ irule exp_alpha_Lam
+      \\ irule exp_alpha_perm_closed
+      \\ last_x_assum irule
+      \\ fs[EXTENSION,SUBSET_DEF] \\ metis_tac[]
+    )
+    \\ irule exp_alpha_Lam
+    \\ last_x_assum irule
+    \\ fs[EXTENSION,SUBSET_DEF] \\ metis_tac[]
+  )
+  THEN1 (
+    fs[avoid_vars_def]
+    \\ irule exp_alpha_App \\ fs[]
+  )
+  \\ fs[avoid_vars_def]
+  \\ ‘freevars e ⊆ set (MAP FST lcs) ∪ set avoid
+      ∪ set (MAP SND
+             (fresh_var_list (nub (FILTER (λx. MEM x avoid) (MAP FST lcs)))
+               (MAP FST lcs ++ avoid)))’ by (
+     fs[EXTENSION,SUBSET_DEF] \\ metis_tac[]
+  )
+  \\ res_tac \\ fs[] \\ rw[]
+  \\ irule exp_alpha_perm_exp_list_trans
+  \\ conj_tac
+  THEN1 (
+    fs[ZIP_MAP]
+    \\ fs[MAP_MAP_o,combinTheory.o_DEF]
+    \\ fs[freevars_perm_exp]
+    \\ fs[MAP_FST_fresh_var_list]
+    \\ fs[MAP_MAP_o,combinTheory.o_DEF]
+    \\ fs[FILTER_MEM_INTERSECTION]
+    \\ fs[EXTENSION,DISJOINT_DEF,freevars_perm_exp] \\ metis_tac[]
+  )
+  \\ conj_tac
+  THEN1 (
+    fs [ZIP_MAP]
+    \\ fs[MAP_MAP_o,combinTheory.o_DEF]
+    \\ drule (GSYM exp_alpha_freevars)
+    \\ disch_tac \\ fs[]
+    \\ irule DISJOINT_UNION_DIFF
+    \\ conj_tac
+    THEN1 (
+      irule DISJOINT_SUBSET
+      \\ qexists_tac ‘set (MAP FST lcs ++ avoid)’
+      \\ conj_tac THEN1 (fs[fresh_var_list_correctness])
+      \\ fs[EXTENSION,SUBSET_DEF] \\ metis_tac[]
+    )
+    \\ irule DISJOINT_SUBSET
+    \\ qexists_tac
+       ‘freevars e
+       ∪ BIGUNION (set (MAP
+           (λx.freevars (avoid_vars (MAP FST lcs
+                                     ++ avoid
+                                     ++  MAP SND
+                                          (fresh_var_list
+                                           (nub (FILTER (λx. MEM x avoid) (MAP FST lcs)))
+                                           (MAP FST lcs ++ avoid))) (SND x)))
+           lcs))’
+    \\ reverse conj_tac THEN1 (fs[EXTENSION,SUBSET_DEF] \\ metis_tac[])
+    \\ fs[DISJOINT_BIGUNION]
+    \\ conj_tac
+    THEN1 (
+      once_rewrite_tac[DISJOINT_SYM]
+      \\ irule DISJOINT_SUBSET
+      \\ qexists_tac ‘set (MAP FST lcs ++ avoid)’
+      \\ conj_tac THEN1 (fs[fresh_var_list_correctness])
+      \\ fs[EXTENSION,SUBSET_DEF] \\ metis_tac[]
+    )
+    \\ fs[MEM_MAP] \\ rw[]
+    \\ last_x_assum (qspec_then ‘x’ assume_tac)
+    \\ Cases_on ‘x’ \\ fs[]
+    \\ pop_assum mp_tac
+    \\ impl_tac \\ fs[]
+    \\ impl_tac
+    THEN1 (
+      irule SUBSET_TRANS
+      \\ qexists_tac ‘BIGUNION (set (MAP (λ(fn,e). freevars e) lcs))’
+      \\ reverse conj_tac THEN1 (fs[EXTENSION,SUBSET_DEF] \\ metis_tac[])
+      \\ irule SUBSET_BIGUNION_I
+      \\ fs[MEM_MAP]
+      \\ qexists_tac ‘(q,r)’ \\ fs[]
+    )
+    \\ disch_tac
+    \\ drule (GSYM exp_alpha_freevars)
+    \\ disch_tac \\ fs[]
+    \\ once_rewrite_tac[DISJOINT_SYM]
+    \\ irule DISJOINT_SUBSET
+    \\ qexists_tac ‘set (MAP FST lcs ++ avoid)’
+    \\ conj_tac THEN1 (fs[fresh_var_list_correctness])
+    \\ fs[]
+    \\ once_rewrite_tac[UNION_SYM]
+    \\ irule DIFF_SUBSET_UNION
+    \\ irule SUBSET_TRANS
+    \\ qexists_tac ‘BIGUNION (set (MAP (λ(fn,e). freevars e) lcs)) DIFF
+                    set (MAP FST lcs)’
+    \\ reverse conj_tac THEN1 (fs[EXTENSION,SUBSET_DEF] \\ metis_tac[])
+    \\ qsuff_tac ‘freevars r ⊆ BIGUNION (set (MAP (λ(fn,e). freevars e) lcs))’
+    THEN1 (fs[EXTENSION,SUBSET_DEF] \\ metis_tac[])
+    \\ irule SUBSET_BIGUNION_I
+    \\ fs[MEM_MAP]
+    \\ qexists_tac ‘(q,r)’ \\ fs[]
+  )
+  \\ fs[ZIP_MAP]
+  \\ fs[MAP_MAP_o,combinTheory.o_DEF]
+  \\ irule exp_alpha_Letrec
+  \\ rw[]
+  THEN1 (fs[MAP_MAP_o,combinTheory.o_DEF,MAP_EQ_f])
+  \\ fs[MAP_MAP_o,combinTheory.o_DEF,MAP_EQ_f]
+  \\ fs[EVERY2_EVERY]
+  \\ fs[ZIP_MAP]
+  \\ fs[MAP_MAP_o,combinTheory.o_DEF,MAP_EQ_f]
+  \\ fs[EVERY_MEM]
+  \\ Cases
+  \\ fs[MEM_MAP]
+  \\ rw[]
+  \\ Cases_on ‘x’ \\ fs[]
+  \\ res_tac \\ fs[]
+  \\ pop_assum irule
+  \\ irule SUBSET_TRANS
+  \\ qexists_tac ‘BIGUNION (set (MAP (λ(fn,e). freevars e) lcs))’
+  \\ reverse conj_tac THEN1 (fs[EXTENSION,SUBSET_DEF] \\ metis_tac[])
+  \\ irule SUBSET_BIGUNION_I
+  \\ fs[MEM_MAP]
+  \\ qexists_tac ‘(q,r)’ \\ fs[]
+QED
+
+
+
+
+(********Capture avoiding substitution**********)
+
+
+
+Definition CA_subst_def:
+   CA_subst x arg body =
+       subst x arg (avoid_vars (freevars arg ++ freevars body) body)
+End
+
+Theorem App_Lam_bisim:
+  closed (Lam x body) ∧ closed arg ⇒
+  App (Lam x body) arg ≃ subst x arg body
+Proof
+  rw [] \\ match_mp_tac eval_IMP_app_bisimilarity
+  \\ fs [eval_Let,bind_single_def]
+  \\ match_mp_tac IMP_closed_subst
+  \\ fs [] \\ fs [closed_def,FILTER_EQ_NIL,EVERY_MEM,SUBSET_DEF]
+QED
+
+Triviality app_bisimilarity_trans:
+  ∀x y z. x ≃ y ∧ y ≃ z ⇒ x ≃ z
+Proof
+  rw[]
+  \\ assume_tac transitive_app_bisimilarity
+  \\ fs[transitive_def]
+  \\ res_tac \\ fs[]
+QED
+
+Triviality app_bisimilarity_sym:
+  ∀x y. x ≃ y ⇒ y ≃ x
+Proof
+  rw[]
+  \\ assume_tac symmetric_app_bisimilarity
+  \\ fs[symmetric_def]
+QED
+
+Theorem freevars_avoid_vars_mono:
+  ∀ avoid e . freevars e ⊆ set avoid
+  ⇒ freevars (avoid_vars avoid e) = freevars e
+Proof
+  rw[]
+  \\ drule exp_alpha_avoid_vars
+  \\ disch_tac
+  \\ imp_res_tac exp_alpha_freevars
+  \\ fs[]
+QED
+
+Theorem boundvars_perm_exp_list:
+  ∀ binds e.
+     ALL_DISTINCT (MAP FST binds)
+  ∧  ALL_DISTINCT (MAP SND binds)
+  ∧  DISJOINT (set (MAP SND binds)) (boundvars e)
+  ⇒  boundvars (perm_exp_list binds e) ⊆
+     boundvars e DIFF (set (MAP FST binds)) ∪ set (MAP SND binds)
+Proof
+  recInduct perm_exp_list_ind
+  \\ conj_tac THEN1 (fs[perm_exp_list_def])
+  \\ rw[]
+  \\ fs[perm_exp_list_def]
+  \\ fs[boundvars_perm_exp]
+  \\ last_x_assum mp_tac
+  \\ reverse impl_tac
+  \\ rw[]
+  \\ fs[EXTENSION,SUBSET_DEF,DISJOINT_DEF] \\ metis_tac[MEM]
+QED
+
+Triviality DISJOINT_UNION_DIFF_DISTRIB:
+  DISJOINT (A ∪ B DIFF C) D ⇔ DISJOINT (A DIFF C) D ∧ DISJOINT (B DIFF C) D
+Proof
+  fs[EXTENSION,DISJOINT_DEF,SUBSET_DEF] \\ metis_tac[]
+QED
+
+Triviality DISJOINT_DIFF_WEAKENING:
+  DISJOINT A B ⇒ DISJOINT (A DIFF C) B
+Proof
+  fs[EXTENSION,DISJOINT_DEF,SUBSET_DEF] \\ metis_tac[]
+QED
+
+Triviality FILTER_MAP_MEM:
+  ∀ l1 l2. MEM x l1 ∧ MEM x l2 ⇒ MEM x (nub (FILTER (λx. MEM x l1) l2))
+Proof
+  Induct_on ‘l1’ \\ fs[]
+  \\ rw[] \\ res_tac \\ fs[]
+  \\ Induct_on ‘l2’ \\ fs[]
+  \\ rw[] \\ res_tac \\ fs[]
+QED
+
+Triviality MEM_PAIR_MAP:
+  MEM (q,r) lcs ⇒ MEM q (MAP FST lcs)
+Proof
+  Induct_on ‘lcs’ \\ fs[]
+  \\ Cases \\ fs[] \\ rw[]
+  \\ res_tac \\ fs[]
+QED
+
+Triviality NOT_MEM_PAIR:
+ (∀y. q ≠ FST y ∨ ¬MEM y l) ⇒ ¬MEM q (MAP FST l)
+Proof
+  Induct_on ‘l’ \\ fs[]
+  \\ Cases \\ fs[] \\ rw[]
+  THEN1 (
+    CCONTR_TAC \\ fs[] \\ rw[]
+    \\ last_x_assum mp_tac
+    \\ impl_tac THEN1 (metis_tac[MEM])
+    \\ fs[]
+    \\ pop_assum (qspec_then ‘(q,r)’ assume_tac) \\ fs[]
+  )
+  \\ last_x_assum irule
+  \\ rw[]
+  \\ pop_assum (qspec_then ‘y’ assume_tac) \\ fs[]
+QED
+
+Triviality NOT_MEM_DISJOINT:
+  ¬MEM x l ⇔ DISJOINT {x} (set l)
+Proof
+  fs[EXTENSION,DISJOINT_DEF] \\ metis_tac[MEM]
+QED
+
+Theorem avoid_vars_safe_renaming:
+  ∀ avoid e . freevars e ⊆ set avoid
+  ⇒ DISJOINT (boundvars (avoid_vars avoid e)) (set avoid)
+Proof
+  recInduct avoid_vars_ind
+  \\ rw[]
+  THEN1 (fs[avoid_vars_def])
+  THEN1 (
+    fs[avoid_vars_def]
+    \\ fs[MAP_MAP_o,combinTheory.o_DEF]
+    \\ fs[LIST_TO_SET_FLAT]
+    \\ fs[MAP_MAP_o,combinTheory.o_DEF]
+    \\ fs[MEM_MAP]
+    \\ fs[BIGUNION_SUBSET]
+    \\ rw[]
+    \\ last_x_assum irule
+    \\ fs[]
+    \\ first_x_assum (qspec_then ‘freevars a’ assume_tac)
+    \\ pop_assum irule
+    \\ fs[MEM_MAP]
+    \\ qexists_tac ‘a’ \\ fs[]
+  )
+  THEN1 (
+    ‘freevars e ⊆ x INSERT fresh_var x avoid INSERT set avoid’ by (
+      fs[EXTENSION,SUBSET_DEF] \\ metis_tac[]
+    )
+    \\ fs[] \\ pop_assum kall_tac
+    \\ fs[avoid_vars_def]
+    \\ rw[] \\ fs[fresh_var_correctness]
+    \\ simp[boundvars_perm_exp]
+    \\ rw[]
+    \\ fs[EXTENSION,DISJOINT_DEF,SUBSET_DEF] \\ metis_tac[fresh_var_correctness]
+  )
+  THEN1 (fs[avoid_vars_def])
+  \\ ‘freevars e ⊆
+        set (MAP FST lcs) ∪ set avoid ∪
+        set (MAP SND
+             (fresh_var_list (nub (FILTER (λx. MEM x avoid) (MAP FST lcs)))
+                (MAP FST lcs ++ avoid)))’ by (
+     fs[EXTENSION,SUBSET_DEF] \\ metis_tac[]
+  )
+  \\ fs[] \\ pop_assum kall_tac
+  \\ qspecl_then [‘(nub (FILTER (λx. MEM x avoid) (MAP FST lcs)))’
+                 ,‘(MAP FST lcs ++ avoid)’] assume_tac fresh_var_list_correctness
+  \\ fs[avoid_vars_def]
+  \\ fs[ZIP_MAP]
+  \\ fs[MAP_MAP_o,combinTheory.o_DEF]
+  \\ once_rewrite_tac[DISJOINT_SYM]
+  \\ irule DISJOINT_SUBSET
+  \\ qspecl_then
+     [‘(fresh_var_list
+                   (nub (FILTER (λx. MEM x avoid) (MAP FST lcs)))
+                   (MAP FST lcs ++ avoid))’
+     ,‘(Letrec
+                   (MAP
+                      (λx.
+                           (FST x,
+                            avoid_vars
+                              (MAP FST lcs ++ avoid ++
+                               MAP SND
+                                 (fresh_var_list
+                                    (nub
+                                       (FILTER (λx. MEM x avoid)
+                                          (MAP FST lcs)))
+                                    (MAP FST lcs ++ avoid))) (SND x))) lcs)
+                   (avoid_vars
+                      (MAP FST lcs ++ avoid ++
+                       MAP SND
+                         (fresh_var_list
+                            (nub (FILTER (λx. MEM x avoid) (MAP FST lcs)))
+                            (MAP FST lcs ++ avoid))) e))’]
+     mp_tac boundvars_perm_exp_list
+  \\ impl_tac
+  THEN1 (
+    fs[MAP_FST_fresh_var_list]
+    \\ conj_tac THEN1 (irule fresh_var_list_distinctness)
+    \\ conj_tac
+    THEN1 (fs[EXTENSION,DISJOINT_DEF,SUBSET_DEF] \\ metis_tac[])
+    \\ fs[MAP_MAP_o,combinTheory.o_DEF]
+    \\ fs[MEM_MAP]
+    \\ rw[]
+    \\ Cases_on ‘x’ \\ fs[]
+    \\ reverse conj_tac
+    THEN1 (
+      once_rewrite_tac[NOT_MEM_DISJOINT]
+      \\ once_rewrite_tac[DISJOINT_SYM]
+      \\ irule DISJOINT_SUBSET
+      \\ qexists_tac ‘set (MAP FST lcs ++ avoid)’
+      \\ fs[fresh_var_list_correctness]
+      \\ metis_tac[MEM_PAIR_MAP,MEM]
+    )
+    \\ res_tac \\ fs[]
+    \\ once_rewrite_tac[DISJOINT_SYM]
+    \\ first_assum irule
+    \\ irule SUBSET_TRANS
+    \\ qexists_tac ‘BIGUNION (set (MAP (λ(fn,e). freevars e) lcs))’
+    \\ reverse conj_tac THEN1 (fs[EXTENSION,SUBSET_DEF] \\ metis_tac[])
+    \\ irule SUBSET_BIGUNION_I
+    \\ fs[MEM_MAP]
+    \\ qexists_tac ‘(q,r)’ \\ fs[]
+  )
+  \\ strip_tac
+  \\ qexists_tac ‘ boundvars
+          (Letrec
+             (MAP
+                (λx.
+                     (FST x,
+                      avoid_vars
+                        (MAP FST lcs ++ avoid ++
+                         MAP SND
+                           (fresh_var_list
+                              (nub (FILTER (λx. MEM x avoid) (MAP FST lcs)))
+                              (MAP FST lcs ++ avoid))) (SND x))) lcs)
+             (avoid_vars
+                (MAP FST lcs ++ avoid ++
+                 MAP SND
+                   (fresh_var_list
+                      (nub (FILTER (λx. MEM x avoid) (MAP FST lcs)))
+                      (MAP FST lcs ++ avoid))) e)) DIFF
+        set
+          (MAP FST
+             (fresh_var_list (nub (FILTER (λx. MEM x avoid) (MAP FST lcs)))
+                (MAP FST lcs ++ avoid))) ∪
+        set
+          (MAP SND
+             (fresh_var_list (nub (FILTER (λx. MEM x avoid) (MAP FST lcs)))
+                (MAP FST lcs ++ avoid)))’
+  \\ fs[]
+  \\ reverse conj_tac THEN1 (
+    irule DISJOINT_SUBSET
+    \\ qexists_tac ‘set (MAP FST lcs ++ avoid)’
+    \\ fs[fresh_var_list_correctness]
+  )
+  \\ fs[DISJOINT_UNION_DIFF_DISTRIB]
+  \\ conj_tac THEN1 (fs[EXTENSION,DISJOINT_DEF,DIFF_DEF] \\ metis_tac[])
+  \\ fs[MAP_MAP_o,combinTheory.o_DEF]
+  \\ fs[pure_miscTheory.BIGUNION_DIFF]
+  \\ GEN_TAC
+  \\ rw[]
+  \\ fs[MEM_MAP]
+  \\ Cases_on ‘x’ \\ fs[] \\ rw[]
+  THEN1 (
+    res_tac \\ fs[]
+    \\ irule DISJOINT_DIFF_WEAKENING
+    \\ once_rewrite_tac[DISJOINT_SYM]
+    \\ first_assum irule
+    \\ irule SUBSET_TRANS
+    \\ qexists_tac ‘ BIGUNION (set (MAP (λ(fn,e). freevars e) lcs))’
+    \\ reverse conj_tac
+    THEN1 (fs[EXTENSION,DISJOINT_DEF,SUBSET_DEF] \\ metis_tac[])
+    \\ irule SUBSET_BIGUNION_I
+    \\ fs[MEM_MAP]
+    \\ qexists_tac ‘(FST y,r)’ \\ fs[]
+  )
+  THEN1 (
+    fs[MAP_FST_fresh_var_list]
+    \\ irule DISJOINT_DIFF_WEAKENING
+    \\ res_tac \\ fs[]
+    \\ once_rewrite_tac[DISJOINT_SYM]
+    \\ first_assum irule
+    \\ irule SUBSET_TRANS
+    \\ qexists_tac ‘BIGUNION (set (MAP (λ(fn,e). freevars e) lcs))’
+    \\ reverse conj_tac THEN1 (fs[EXTENSION,SUBSET_DEF] \\ metis_tac[])
+    \\ irule SUBSET_BIGUNION_I
+    \\ fs[MEM_MAP]
+    \\ qexists_tac ‘(q,r)’ \\ fs[]
+  )
+  \\ fs[]
+  \\ ‘¬MEM q (MAP FST (fresh_var_list (nub (FILTER (λx. MEM x avoid) (MAP FST lcs)))
+                      (MAP FST lcs ++ avoid)))’ by (
+     irule NOT_MEM_PAIR \\ fs[]
+  )
+  \\ CCONTR_TAC \\ fs[]
+  \\ ‘MEM q (nub (FILTER (λx. MEM x avoid) (MAP FST lcs)))’ by (
+    irule FILTER_MAP_MEM
+    \\ fs[]
+    \\ drule MEM_PAIR_MAP \\ fs[]
+  )
+  \\ ‘MEM q (MAP FST (fresh_var_list (nub (FILTER (λx. MEM x avoid) (MAP FST lcs)))
+                     (MAP FST lcs ++ avoid)))’ by (
+       qspecl_then [‘(nub (FILTER (λx. MEM x avoid) (MAP FST lcs)))’
+                   ,‘(MAP FST lcs ++ avoid)’] assume_tac MAP_FST_fresh_var_list
+       \\ metis_tac[MEM]
+     )
+  \\ fs[]
+QED
+
+Theorem boundvars_avoid_vars:
+∀l x. freevars body ⊆ set l ∧
+      MEM x (boundvars (avoid_vars l body)) ⇒
+        ¬MEM x l
+Proof
+  rw[]
+  \\ qspecl_then [‘l’,‘body’] assume_tac avoid_vars_safe_renaming
+  \\ res_tac
+  \\ fs[EXTENSION,DISJOINT_DEF] \\ metis_tac[MEM]
+QED
+
+Theorem subst_NOT_MEM:
+ ∀ f arg.  ¬MEM n (freevars arg) ⇒ subst (f \\ n) arg = subst f arg
+Proof
+  recInduct subst_ind
+  \\ rw[]
+  THEN1 (fs[subst_def,DOMSUB_FLOOKUP_NEQ])
+  THEN1 (
+    fs[subst_def]
+    \\ fs[MAP_EQ_f]
+    \\ rw[] \\ res_tac \\ fs[]
+    \\ pop_assum irule
+    \\ fs[MEM_MAP] \\ metis_tac[MEM]
+  )
+  THEN1 (
+    fs[subst_def] \\ res_tac \\ fs[]
+  )
+  THEN1 (
+    fs[subst_def]
+    \\ fs[DOMSUB_COMMUTES]
+  )
+  THEN1 (
+    fs[subst_def]
+  )
+  THEN1 (
+    res_tac \\ fs[] \\ rw[]
+    \\ fs[subst_def]
+    \\ reverse conj_tac THEN1 (fs[fdiff_fdomsub_commute])
+    \\ fs[MEM_MAP]
+    \\ fs[MAP_EQ_f] \\ rw[]
+    \\ Cases_on ‘e’ \\ fs[]
+    \\ res_tac
+    \\ fs[fdiff_fdomsub_commute]
+    \\ pop_assum irule
+    \\ first_assum (qspec_then ‘freevars r’ assume_tac) \\ fs[]
+    \\ pop_assum (qspec_then ‘(q,r)’ assume_tac) \\ fs[]
+  )
+  \\ fs[subst_def]
+  \\ fs[fdiff_fdomsub_INSERT]
+  \\ ‘n INSERT set (MAP FST f) = set (MAP FST f)’ by (
+    fs[EXTENSION] \\ metis_tac[MEM]
+  )
+  \\ fs[]
+QED
+
+Triviality MAP_FST_list_mono:
+  ∀ g l. MAP (λx. FST ((λ(f,e).(f,g e)) x)) l = MAP FST l
+Proof
+  rw[] \\ fs[MAP_EQ_f] \\ Cases \\ fs[]
+QED
+
+Triviality MAP_FST_MEM_pair_companion:
+  ∀x. MEM x (MAP FST lcs) ⇒ ∃ y. MEM (x,y) lcs
+Proof
+  rw[]
+  \\ Induct_on ‘lcs’ \\ fs[]
+  \\ Cases \\ fs[]
+  \\ Cases_on ‘x = q’ \\ fs[] \\ rw[]
+  \\ qexists_tac ‘r’ \\ fs[]
+QED
+
+Triviality INSERT_absorption:
+  MEM x l ⇒ x INSERT (set l) = set l
+Proof
+  fs[EXTENSION] \\ metis_tac[]
+QED
+
+Theorem subst_distrib:
+  ∀ body f v arg.
+    (∀n v. FLOOKUP f n = SOME v ⇒ closed v)
+  ∧ EVERY (λ x. x ∉ freevars arg) (boundvars body)
+   ⇒
+  subst f (subst v arg body)
+  = subst v (subst f arg) (subst (f \\ v) body)
+Proof
+  ho_match_mp_tac freevars_ind
+  \\ rpt strip_tac
+  THEN1(
+    fs[subst_def]
+    \\ fs[FLOOKUP_UPDATE] \\ fs[DOMSUB_FLOOKUP_THM]
+    \\ rw[] \\ fs[subst_single_def]
+    \\ Cases_on ‘FLOOKUP f n’ \\ fs[subst_single_def] \\ fs[subst_def]
+    \\ res_tac \\ fs[closed_subst])
+  THEN1(
+    fs[subst_def]
+    \\ fs[MAP_MAP_o,combinTheory.o_DEF]
+    \\ fs[MAP_EQ_f]
+    \\ fs[EVERY_FLAT,EVERY_MAP,EVERY_MEM]
+    \\ rw[] \\ res_tac \\ fs[]
+  )
+  THEN1(
+    fs[subst_def]
+    \\ res_tac \\ fs[]
+  )
+  THEN1(
+    fs[subst_single_def]
+    \\ IF_CASES_TAC \\ fs[subst_def]
+    \\ ‘∀m v. FLOOKUP (f \\ n) m = SOME v ⇒ closed v’ by (
+       fs[DOMSUB_FLOOKUP_THM]
+       \\ metis_tac[]
+    )
+    \\ last_x_assum drule
+    \\ disch_then (qspecl_then [‘v’,‘arg’] mp_tac)
+    \\ impl_tac
+    \\ rw[]
+    \\ fs[DOMSUB_FUPDATE_NEQ]
+    \\ fs[subst_NOT_MEM]
+    \\ metis_tac[DOMSUB_COMMUTES]
+  )
+  \\ fs[MAP_MAP_o,combinTheory.o_DEF]
+  \\ fs[EVERY_FLAT,EVERY_MAP,EVERY_MEM]
+  \\ ‘∀ x. MEM x (MAP FST lcs) ⇒ ¬ MEM x (freevars arg)’ by (
+      rw[]
+      \\ last_assum irule
+      \\ imp_res_tac MAP_FST_MEM_pair_companion
+      \\ res_tac
+      \\ qexists_tac ‘(x,y)’ \\ fs[]
+  )
+  \\ fs[subst_def]
+  \\ fs[MAP_MAP_o,combinTheory.o_DEF]
+  \\ fs[MAP_FST_list_mono]
+  \\ fs[MAP_EQ_f]
+  \\ rw[]
+  \\ TRY (Cases_on ‘x’ \\ fs[])
+  \\ ‘(FDIFF (f \\ v) (set (MAP FST lcs))) = (FDIFF f (set (MAP FST lcs))) \\ v’ by (
+     simp[Once fdiff_fdomsub_commute]
+  ) \\ fs[] \\ pop_assum kall_tac
+  \\ ‘subst f arg = subst (FDIFF f (set (MAP FST lcs))) arg’ by (
+     irule subst_FDIFF'' \\ fs[]
+  ) \\ fs[] \\ pop_assum kall_tac
+  THEN1 (
+    last_x_assum (qspecl_then [‘q’,‘r’] mp_tac) \\ fs[]
+    \\ disch_tac
+    \\ simp[FDIFF_def]
+    \\ rw[]
+    \\ simp[GSYM FDIFF_def]
+    THEN1 (
+      first_assum irule
+      \\ rw[]
+      THEN1 (
+        first_assum irule
+        \\ qexists_tac ‘n’
+        \\ irule FLOOKUP_SUBMAP
+        \\ qexists_tac ‘(FDIFF f (set (MAP FST lcs)))’ \\ fs[]
+        \\ fs[FDIFF_def,DRESTRICT_SUBMAP]
+      )
+      \\ last_assum irule
+      \\ qexists_tac ‘(q,r)’ \\ fs[]
+    )
+    \\ once_rewrite_tac[GSYM fdiff_fdomsub_commute]
+    \\ fs[fdiff_fdomsub_INSERT]
+    \\ fs[INSERT_absorption]
+  )
+  \\ simp[FDIFF_def]
+  \\ rw[]
+  \\ simp[GSYM FDIFF_def]
+  THEN1 (
+    first_assum irule
+    \\ rw[]
+    \\ first_assum irule
+    \\ qexists_tac ‘n’
+    \\ irule FLOOKUP_SUBMAP
+    \\ qexists_tac ‘(FDIFF f (set (MAP FST lcs)))’ \\ fs[]
+    \\ fs[FDIFF_def,DRESTRICT_SUBMAP]
+  )
+  \\ once_rewrite_tac[GSYM fdiff_fdomsub_commute]
+  \\ fs[fdiff_fdomsub_INSERT]
+  \\ fs[INSERT_absorption]
+QED
+
+Theorem beta_equivalence:
+  App (Lam x body) arg ≅ CA_subst x arg body
+Proof
+  fs[CA_subst_def]
+  \\ fs[exp_eq_def]
+  \\ rpt strip_tac
+  \\ fs[bind_def]
+  \\ rw[]
+  \\ fs[subst_def]
+  \\ match_mp_tac app_bisimilarity_trans
+  \\ qexists_tac ‘ subst x (subst f arg) (subst (f \\ x) body)’
+  \\ conj_tac
+  THEN1 (
+    irule App_Lam_bisim
+    \\ conj_tac THEN1 (
+      irule IMP_closed_subst \\ fs[FRANGE_DEF]
+      \\ fs[FLOOKUP_DEF,PULL_EXISTS]
+    )
+    \\ qsuff_tac ‘closed (subst f (Lam x body))’ THEN1 (fs[subst_def])
+    \\ irule IMP_closed_subst \\ fs[FRANGE_DEF]
+    \\ fs[FLOOKUP_DEF,PULL_EXISTS]
+  )
+  \\ drule subst_distrib
+  \\ disch_then (qspecl_then [‘(avoid_vars (freevars arg ++ freevars body) body)’
+                             ,‘x’,‘arg’] mp_tac)
+  \\ impl_tac
+  THEN1 (
+    fs[EVERY_MEM]
+    \\ rw[]
+    \\ imp_res_tac boundvars_avoid_vars \\ fs[]
+  )
+  \\ rw[]
+  \\ ‘(∀v. v ∈ FRANGE (f \\ x) ⇒ closed v)’ by (
+    rw[]
+    \\ first_assum irule
+    \\ fs[GSYM IN_FRANGE_FLOOKUP]
+    \\ fs[EXTENSION,FRANGE_DEF,IN_DEF] \\ rw[]
+    \\ fs[DOMSUB_FAPPLY_THM] \\ rw[]
+    \\ metis_tac[]
+  )
+  \\ fs[subst_subst_FUNION]
+  \\ irule app_bisimilarity_sym
+  \\ irule exp_alpha_app_bisimilarity
+  \\ reverse (rpt conj_tac)
+  THEN1 (
+    irule exp_alpha_subst_all_closed''
+    \\ rw[]
+    THEN1 (
+      qspecl_then [‘FEMPTY |+ (x,subst f arg)’,‘f \\ x’] mp_tac (GEN_ALL FRANGE_FUNION)
+      \\ impl_tac THEN1 (fs[FDOM_DOMSUB])
+      \\ disch_tac \\ fs[] \\ pop_assum kall_tac
+      \\ rw[]
+      \\ irule IMP_closed_subst \\ fs[]
+      \\ rw[]
+      \\ last_assum irule
+      \\ fs[GSYM IN_FRANGE_FLOOKUP]
+    )
+    \\ fs[exp_alpha_sym,exp_alpha_avoid_vars]
+  )
+  \\ irule IMP_closed_subst \\ fs[]
+  \\ rw[]
+  \\ TRY (
+    qspecl_then [‘FEMPTY |+ (x,subst f arg)’,‘f \\ x’] mp_tac (GEN_ALL FRANGE_FUNION)
+    \\ impl_tac THEN1 (fs[FDOM_DOMSUB])
+    \\ disch_tac \\ fs[] \\ pop_assum kall_tac
+    \\ rw[]
+    \\ irule IMP_closed_subst \\ fs[]
+    \\ rw[]
+    \\ last_assum irule
+    \\ fs[GSYM IN_FRANGE_FLOOKUP]
+  )
+  \\ fs[freevars_avoid_vars_mono]
+  \\ fs[EXTENSION,SUBSET_DEF] \\ metis_tac[]
+QED
+
+
+val _ = export_theory();
